Tests/STLC/TrmSpec.lean
@@ -17,11 +17,11 @@ class TestEnv where
 
 variable [testEnv : TestEnv]
 
-@[reducible] instance core : EnvCore := { D := String, uid2val := testEnv.trm2val }
-@[reducible] instance env : ExeEnv core := { uid2valCtx := testEnv.trm2valCtx }
+@[reducible] instance refs : ExeRefs := { D := String, uid2val := testEnv.trm2val }
+@[reducible] instance env : ExeEnv refs := { uid2valCtx := testEnv.trm2valCtx }
 
-def upcast {l : Label} (self : AST Symbolic.I l) : AST core.ExeParameters l :=
-  self.map (F := Symbolic.I) (G := core.ExeParameters) (λ (s : Symbol) => nomatch s) id
+def upcast {l : Label} (self : AST Symbolic.I l) : AST refs.ExeParameters l :=
+  self.map (F := Symbolic.I) (G := refs.ExeParameters) (λ (s : Symbol) => nomatch s) id
 
 attribute [local simp] AST.eval AST.map upcast
 attribute [local simp] Trm.vFalse Trm.vTrue Trm.primitiveIdFn Trm.primitiveIdFnOnFalse
@@ -79,16 +79,16 @@ end eval
 
 section compilerCapability
 
-variable [compilerCore : EnvCore] [build : BuildEnv compilerCore]
+variable [refs : ExeRefs] [build : BuildEnv refs]
 
 example : True := by
   fail_if_success
-    have _receipt := compilerCore.uid2val.inv
+    have _receipt := refs.uid2val.inv
   trivial
 
 example : True := by
   fail_if_success
-    have _exe : ExeEnv compilerCore := inferInstance
+    have _exe : ExeEnv refs := inferInstance
   trivial
 
 end compilerCapability
